---
title: "On The Irrationality of Apery's Constant"
date: 2024-04-15
permalink: /posts/2025/04/apery/
tags:
  - complex analysis
  - number theory
---

Abstract
-----
I will discuss the bizarre proof that the constant \\( \zeta(3) \\) (known as Apery's constant) is irrational.

Introduction
=====
The Riemann zeta function is the unique analytic continuation of the function \\(\zeta(s) = \sum_\{n \geq 1\} \frac{1}{n^s}\\) (a priori defined only on \\(s \in \mathbb{R} \times i \mathbb{R}_+ \\) ) to the whole complex plane. Naturally, as the subject of the Riemann hypothesis, the zeta function is one of the most well-known functions in mathematics. It turns out that despite extremely being well-studied, we still don't know basic things about \\(\zeta(s) \\). It is not too hard to show that

$$
\begin{align*} 
\zeta( -2k) = 0 & \qquad \forall k \in \mathbb{N},\\
\zeta( -2k + 1 ) \in \mathbb{Q} & \qquad \forall k \in \mathbb{N},\\
\zeta( 2k ) \in \pi^{2k}\mathbb{Q} & \qquad \forall k \in \mathbb{N} \cup \set{ 0 }.
\end{align*}
$$

Hence we know the irrationality of \\(\zeta(k)\\) when \\( k \\) is an integer that isn't odd and positive. One would very much expect from the above that \\( \zeta(2k + 1) \in \pi^{2k+1} \mathbb{Q} \\), but we have no idea. Even worse we have no idea if in general \\( \zeta(2k+1) \in \mathbb{R} \setminus \mathbb{Q} \\)! It took many years until very recently (in 1978) Apery showed that \\[ \zeta(3) \in \mathbb{R} \setminus \mathbb{Q}. \\]

This proof is quite notable for two main reasons. Firstly the proof uses no "advanced" techniques, and could have been replicated hundreds of years ago by Riemann. Secondly the proof has resisted any and all (to my knowledge) attempts to be adapted for other results.

How Is It Done?
=====

Apery used the following result

<i> hello hello \\( asd \int \\) hello \\[ heloo \\] hello $$ hello $$ hello <\i>

<b>Lemma</b>: Suppose that \\[ asd.\\] Then it is true that. 

```
hello world \\( f(x) = \int \\)

$\int$

$$\int$$
```



References
-----
Almost all of this is derived from Van de Poorten's article on the matter. 

$$
\displaylines{
\nabla \cdot E= \frac{\rho}{\epsilon_0} \\\
\nabla \cdot B=0 \\\
\nabla \times E= -\partial_tB \\\
\nabla \times B  = \mu_0 \left(J + \varepsilon_0 \partial_t E \right)
}
$$
